src/Decidables.v
@@ -1,0 +1,83 @@
+Require Import List EqdepClass.
+Require Export EquivDec.
+
+Set Implicit Arguments.
+Set Strict Implicit.
+
+Theorem EquivDec_refl_left (T : Type) {c : EqDec T (@eq T)} :
+  forall (n : T), equiv_dec n n = left (refl_equal _).
+Proof.
+  intros. destruct (equiv_dec n n); try congruence.
+  Require Eqdep_dec.
+  rewrite (Eqdep_dec.UIP_dec (A := T) (@equiv_dec _ _ _ c) e (refl_equal _)).
+  reflexivity.
+Qed.
+
+Class SemiDec (t : Type) : Type :=
+{ seq_dec : forall a b : t, option (a = b) }.
+Global Instance EquivDec_SemiDec t (EQ : EqDec t (@eq t)) : SemiDec t :=
+{ seq_dec := fun a b =>
+  match equiv_dec a b with
+    | left pf => Some pf
+    | right _ => None
+  end 
+}.
+
+Global Instance EquivDec_nat : EqDec nat (@eq nat) :=
+  Peano_dec.eq_nat_dec.  
+
+Global Instance SemiDec_option T (S : SemiDec T) : SemiDec (option T) :=
+{ seq_dec := fun a b =>
+  match a as a, b as b return option (a = b) with
+    | None , None => Some (refl_equal _)
+    | Some x , Some y => 
+      match seq_dec x y with
+        | None => None
+        | Some pf => 
+          match pf in _ = t return option (Some x = Some t) with
+            | refl_equal => Some (refl_equal _)
+          end
+      end
+    | _ , _ => None
+  end
+}.
+
+Global Instance SemiDec_list T (S : SemiDec T) : SemiDec (list T) :=
+{ seq_dec := fix seq_dec' a b : option (a = b) :=
+  match a as a, b as b return option (a = b) with
+    | nil , nil => Some (refl_equal _)
+    | x :: xs , y :: ys => 
+      match seq_dec x y with
+        | None => None
+        | Some pf => 
+          match seq_dec' xs ys with
+            | None => None
+            | Some pf' => 
+              match pf in _ = t , pf' in _ = t' return option (x :: xs = t :: t') with
+                | refl_equal , refl_equal => Some (refl_equal _)
+              end
+          end
+      end
+    | _ , _ => None
+  end
+}.
+
+Inductive dcomp T (a b : T) : Type :=
+| Lt | Gt | Eq : a = b -> dcomp a b.
+
+Class Comparable (t : Type) : Type :=
+{ cmp_dec : forall a b : t, dcomp a b }.
+Class SemiComparable (t : Type) : Type :=
+{ scmp_dec : forall a b : t, option (dcomp a b) }.
+Global Instance Comparable_SemiComparable t (SC : Comparable t) 
+  : SemiComparable t :=
+{ scmp_dec := fun a b => Some (cmp_dec a b) }.
+
+Global Instance Comparable_nat : Comparable nat :=
+{| cmp_dec :=
+   fun a b => match Compare_dec.lt_eq_lt_dec a b with
+                | inleft (left _) => Lt _ _
+                | inleft (right pf) => Eq pf
+                | inright _ => Gt _ _
+              end
+|}.
